src/rocq/Semantics/Operations.v
@@ -1,0 +1,15 @@
+From Vellvm Require Import
+  Semantics.LLVMParams
+  Semantics.Gep
+  Semantics.Select
+  Semantics.Compare
+  Semantics.Conversion
+  Semantics.Memory.MemoryBytes.
+
+Module Operations (LP : LLVMParams).
+  Module GEP     := Gep.GEP LP.
+  Module SELECT  := Select.SELECT LP.
+  Module COMPARE := Compare.COMPARE LP.
+  Module MBYTES  := MemoryBytes.Make LP.
+  Module CONVERT := Conversion.CONVERT LP MBYTES.
+End Operations.
