src/rocq/Semantics/Select.v
@@ -1,0 +1,55 @@
+From Vellvm Require Import
+  Utilities
+  Syntax
+  Semantics.LLVMParams.
+
+Module SELECT (LP:LLVMParams).
+  Import LP.DV.
+
+  Definition eval_select
+    (cnd : dvalue) (v1 v2 : dvalue) : EOB dvalue
+    := match cnd with
+       | DVALUE_Poison t =>
+           (* TODO: Should be the type of the result of the select... *)
+           ret (DVALUE_Poison t)
+       | @DVALUE_I 1 i =>
+           if (@Integers.unsigned 1 i =? 1)%Z
+           then ret v1
+           else ret v2
+       | DVALUE_Vector _ conds =>
+           let fix loop conds xs ys : EOB (list dvalue) :=
+             match conds, xs, ys with
+             | [], [], [] => ret []
+             | (c::conds), (x::xs), (y::ys) =>
+                 selected <- match c with
+                            | DVALUE_Poison t =>
+                                (* TODO: Should be the type of the result of the select... *)
+                                ret (DVALUE_Poison t)
+                            | @DVALUE_I 1 i =>
+                                if (@Integers.unsigned 1 i =? 1)%Z
+                                then ret x
+                                else ret y
+                            | _ => raise_error "concretize_uvalueM: ill-typed select, condition in vector was not poison or i1."
+                            end;;
+                 rest <- loop conds xs ys;;
+                 ret (selected :: rest)
+             | _, _, _ => raise_error "concretize_uvalueM: ill-typed vector select, length mismatch."
+             end in
+           (* TODO: lazily concretize these vectors to avoid
+                   evaluating elements that aren't chosen? *)
+           match v1, v2 with
+           | DVALUE_Poison t, _ =>
+               (* TODO: Should we make sure t is a vector type...? *)
+               ret (DVALUE_Poison t)
+           | DVALUE_Vector _ _, DVALUE_Poison t =>
+               (* TODO: Should we make sure t is a vector type...? *)
+               ret (DVALUE_Poison t)
+           | DVALUE_Vector t xs, DVALUE_Vector _ ys =>
+               selected <- loop conds xs ys;;
+               ret (DVALUE_Vector t selected)
+           | _, _ => raise_error "concretize_uvalueM: ill-typed vector select, non-vector arguments"
+           end
+       | _ => raise_error "concretize_uvalueM: ill-typed select."
+       end.
+
+End SELECT.
